setting up implementation of HandshakeLogLow and implementing the create API

src/tls/HandshakeLogLow.fst
@@ -11,267 +11,40 @@ module B = LowStar.Buffer
 
 module C = TLSConstants
 module Hash = Hashing
-module HashSpec = Hashing.Spec
 module HSM = HandshakeMessages
 
 module LP = LowParse.Low.Base
 
 module IncHash = EverCrypt.Hash.Incremental
 
-#reset-options "--max_fuel 0 --max_ifuel 0 --using_facts_from '* -LowParse'"
+open HandshakeLog.Common
 
-
-/// Its corresponding format_hs_msg is in the .fsti
-/// These will be implemented using the high-level parsers and serializers from LowParse
-
-assume
-val parse_hs_msg (b:hbytes) : GTot (option HSM.hs_msg)
-
-
-// AR: 1/23: implemented in the .fsti now (was needed for hashing spec)
-
-// /// Bytes from the transcript
-
-// let transcript_bytes (ts:hs_transcript)
-//   : GTot bytes
-//   = admit() //Need to use LowParse spec formatters
-
-
-//buffer and in index into it
-let index (max:uint_32) = i:uint_32{i <= max}
-
-noeq
-type indexed_buf = {
-  len:uint_32;
-  buf:lbuffer8 len;
-  idx:(p:B.pointer (index len){B.disjoint buf p});
-
-  // AR: 1/23: as per most recent discussions, hashing state is kept in HS, HSL is stateless as far as hashing is concerned
-
-  // hash_idx:(p:B.pointer (index len) {
-  //   B.all_disjoint [B.loc_buffer buf;
-  //                   B.loc_buffer idx;
-  //                   B.loc_buffer p]
-  // })
-}
-
-// AR: 1/23: same comment as above, commenting hashing index
-
-unfold
-let loc_indexed_buf_indices i = B.loc_buffer i.idx
-  // B.(loc_union_l [loc_buffer i.idx;
-  //    loc_buffer i.hash_idx])
-
-unfold
-let loc_indexed_buf i = B.(loc_union_l [loc_indexed_buf_indices i;
-                                        loc_buffer i.buf])
-
-let empty_transcript : hs_transcript = []
-
-
-// AR: 1/23: this also seems like it is trying to keep some hashing state?
-//           instead we could just keep an erased list?
-
-// noeq
-// type tx (#max_i:uint_32) (#max_j:uint_32) : i:index max_i -> j:index max_j -> hs_transcript -> Type0 =
-//   | Nil : tx #max_i #max_j 0ul 0ul empty_transcript
-
-//   | IFrag : #i:index max_i ->
-//             #j:index max_j ->
-//             #msgs:hs_transcript ->
-//             tl:tx i j msgs ->
-//             k:index max_i{i < k} ->
-//             msg:HSM.hs_msg{valid_transcript (msg::msgs)} ->
-//             tx k j (msg::msgs)
-
-//   | OFrag : #i:index max_i ->
-//             #j:index max_j ->
-//             #msgs:hs_transcript ->
-//             tl:tx i j msgs ->
-//             k:index max_j{j < k} ->
-//             msg:HSM.hs_msg{valid_transcript (msg::msgs)} ->
-//             tx i k (msg::msgs)
-
-// let tx_repr max_i max_j = i:index max_i & j:index max_j & msgs:hs_transcript & tx i j msgs
-// let tx_repr_ptr max_i max_j = B.pointer (G.erased (tx_repr max_i max_j))
+#reset-options "--max_fuel 0 --max_ifuel 0 --using_facts_from '* -LowParse -FStar.Tactics -FStar.Reflection'"
 
 noeq
 type hsl_state = {
-  input:indexed_buf;
-
-  // AR: 1/23: it seems like we don't maintain any invariants for the output buffer, could we just keep it out of (low) HSL?
-  //output:indexed_buf;
-
-  // AR: 1/23: changing it to a dependent tuple, not low-level?
-  //hash_alg: B.pointer (option Hash.alg);
-
-  hash_state: B.pointer (option (a:Hash.alg & IncHash.state a));
-
-  tx: (p:B.pointer (G.erased hs_transcript){B.all_disjoint [loc_indexed_buf input;
-                                                            B.loc_buffer hash_state;
-                                                            B.loc_buffer p]})
-							    
-
-  // AR: 1/23: trying to simplify a bit, by removing hash state
-
-  // tx: (p:tx_repr_ptr input.len output.len{
-  //   B.(all_disjoint [loc_indexed_buf input;
-  //                    loc_indexed_buf output;
-  //                    loc_buffer hash_alg;
-  //                    loc_buffer p])
-  //  })
+  rgn:Mem.rgn;
+  from_to:B.pointer (option range_t);
+  parsed_bytes:(p:B.pointer (G.erased hbytes){
+    B.(loc_disjoint (loc_buffer from_to) (loc_buffer p)) /\
+    rgn `region_includes` B.(loc_union (loc_buffer from_to) (loc_buffer p))
+  });
 }
 
-let indexed_buf_liveness (h:HS.mem) (i:indexed_buf) =
-  B.live h i.buf /\
-  B.live h i.idx
-  // AR: 1/23: as per comments above, commenting hash state
-  //B.live h i.hash_idx
+let region_of s = s.rgn
 
-let hsl_input_buf_len s = s.input.len
-let hsl_input_buf s = s.input.buf
-let hsl_input_index s h = B.deref h s.input.idx
+let index_from_to s h = B.deref h s.from_to
 
-// AR: 1/23: commenting as part of removing hash-based state
-// let hsl_input_hash_index h s = B.deref h s.input.hash_idx
+let parsed_bytes s h = G.reveal (B.deref h s.parsed_bytes)
 
+let invariant s h =
+  B.live h s.from_to /\ B.live h s.parsed_bytes
 
-// AR: 1/23: commenting as part of removing output state
-// let hsl_output_buf_len (s:hsl_state) = s.output.len
-// let hsl_output_buf (s:hsl_state) = s.output.buf
-// let hsl_output_index h s = B.deref h s.output.idx
-// let hsl_output_hash_index h s = B.deref h s.output.hash_idx
+let footprint s = B.(loc_union (loc_buffer s.from_to) (loc_buffer s.parsed_bytes))
 
-let hsl_local_footprint s h =
-  B.loc_union_l [loc_indexed_buf_indices s.input;
+let frame_hsl_state _ _ _ _ = ()
 
-                 // AR: 1/23: commenting out as part of removing output related state
-                 // loc_indexed_buf_indices s.output;
-		 
-                 B.loc_buffer s.hash_state;
-
-                 (match B.deref h s.hash_state with
-                  | None -> B.loc_none
-		  | Some (| _, hash_st |) -> IncHash.footprint hash_st h);
-
-                 B.loc_buffer s.tx]
-
-/// Handshake can write if all the input messages have been hashed
-
-// AR: 1/23: this is still not clear. HSL is not maintaining any hashing state now
-//           and we have also discussed if this is needed at all
-//           (we are not proving, as of now, anything about state machines of two ends being synchronized)
-let writing h s = true
-  //hsl_input_hash_index h s = hsl_input_index h s
-
-let hash_alg s h =
-  match B.deref h s.hash_state with
-  | None -> None
-  | Some (| a, _ |) -> Some a
-
-
-// AR: 1/23: commenting as part of hash state cleanup
-// let get_tx_repr h s : GTot (tx_repr (hsl_input_buf_len s) (hsl_output_buf_len s)) =
-//   G.reveal (B.deref h s.tx)
-
-let transcript s h = G.reveal (B.deref h s.tx)
-  // let (| _, _, msgs, _ |) = get_tx_repr h s in
-  // msgs
-
-// AR: 1/23: commenting to simplify some hash-related state
-
-// let tx_input_index h s : GTot (index (hsl_input_buf_len s)) =
-//   let (| i, _, msgs, _ |) = get_tx_repr h s in
-//   i
-
-// let tx_output_index h s : GTot (index (hsl_output_buf_len s)) =
-//   let (| _, j, msgs, _ |) = get_tx_repr h s in
-//   j
-
-// let get_tx h s : GTot (tx (tx_input_index h s) (tx_output_index h s) (transcript h s)) =
-//   let (| i, j, msgs, tx |) = get_tx_repr h s in
-//   tx
-
-// #push-options "--initial_ifuel 1 --max_ifuel 1"
-// let msg_correspondence (msg:HSM.hs_msg) (b:Bytes.bytes) (from:index (Bytes.len b)) (to:index (Bytes.len b){from < to}) =
-//     let x = Bytes.sub b from (to - from) in
-//     let popt = parse_hs_msg x in
-//     Some? popt /\
-//     Some?.v popt == msg
-
-// let rec transcript_correspondence
-//           #max_i #max_j
-//           (input:Bytes.bytes)
-//           (output:Bytes.bytes)
-//           (#i:index max_i {i <= Bytes.len input})
-//           (#j:index max_j {j <= Bytes.len output})
-//           #msgs
-//           (tx:tx i j msgs)
-//    : GTot prop
-//           (decreases tx)
-//    = match tx with
-//      | Nil ->    //nothing hashed yet
-//        True
-
-//      | IFrag #_ #_ #from tl to msg ->
-//        msg_correspondence msg input from to /\
-//        transcript_correspondence input output tl
-
-//      | OFrag #_ #_ #_ #from tl to msg ->
-//        msg_correspondence msg output from to /\
-//        transcript_correspondence input output tl
-
-// let indexed_buf_bytes (h:HS.mem) (i:indexed_buf)
-//   : GTot (b:Bytes.bytes{Bytes.len b = B.deref h i.hash_idx})
-//   = Bytes.hide (B.as_seq h (B.gsub i.buf 0ul (B.deref h i.hash_idx)))
-
-let format_hs_msg m = admit ()  //implement in .fsti with LowParse
-
-let hsl_invariant s h =
-  indexed_buf_liveness h s.input /\
-
-  // AR: 1/23: commented as part of removing output state
-  // indexed_buf_liveness h s.output /\
- 
-  B.live h s.hash_state /\
-  B.live h s.tx /\
-
-  hsl_input_index s h <= hsl_input_buf_len s /\
-
-  (match B.deref h s.hash_state with
-   | None -> True
-   | Some (| a, hash_st |) ->
-     //IncHash.hashes already includes the invariant of hash
-     IncHash.hashes #a h hash_st (transcript_bytes (G.reveal (B.deref h s.tx))) /\
-
-     //disjointness of hash footprint from everything else
-     (let hash_fp = IncHash.footprint hash_st h in
-      B.(loc_disjoint hash_fp (loc_indexed_buf s.input) /\
-         loc_disjoint hash_fp (loc_buffer s.hash_state) /\
-	 loc_disjoint hash_fp (loc_buffer s.tx))))
-
-   
-
-  // AR: 1/23: commented as part of removing hash-based state
-
-  // hsl_input_hash_index h s <= hsl_input_index h s /\
-  // hsl_output_hash_index h s <= hsl_output_index h s /\
-  // hsl_input_hash_index h s == tx_input_index h s /\
-  // hsl_output_hash_index h s == tx_output_index h s /\
-  // transcript_correspondence (indexed_buf_bytes h s.input)
-  //                           (indexed_buf_bytes h s.output)
-  //                           #(tx_input_index h s)
-  //                           #(tx_output_index h s)
-  //                           #(transcript h s)
-  //                           (get_tx h s)
-
-let elim_hsl_invariant st h =
-  match B.deref h st.hash_state with
-  | None -> ()
-  | Some (| _, _ |) -> ()
-
-let frame_hsl_state s h0 h1 l = admit ()
-
-#push-options "--max_fuel 0 --max_ifuel 0 --z3rlimit_factor 2"
-let frame_hsl_invariant s h0 h1 l = admit ()
-#pop-options
+let create r =
+  let from_to = B.malloc r None 1ul in
+  let parsed_bytes = B.malloc r (G.hide (Seq.empty)) 1ul in
+  { rgn = r; from_to = from_to; parsed_bytes = parsed_bytes }
